{-# OPTIONS --prop --postfix-projections --safe #-}

module commutative-monoid where

open import Level
open import Data.Unit using (tt)
open import Data.Product using (_,_; projâ‚; projâ‚‚)
open import prop
open import prop-setoid
  using (Setoid; IsEquivalence; idS; _âˆ˜S_; âŠ—-setoid; ğŸ™; module â‰ˆ-Reasoning)
  renaming (_â‡’_ to _â‡’s_; _â‰ƒm_ to _â‰ƒs_; â‰ƒm-isEquivalence to â‰ƒs-isEquivalence)

------------------------------------------------------------------------------
-- Commutative Monoid structure on setoids
--
record CommutativeMonoid {o e} (A : Setoid o e) : Set (o âŠ” e) where
  open Setoid A
  field
    Îµ   : Carrier
    _+_ : Carrier â†’ Carrier â†’ Carrier
    +-cong  : âˆ€ {xâ‚ xâ‚‚ yâ‚ yâ‚‚} â†’ xâ‚ â‰ˆ xâ‚‚ â†’ yâ‚ â‰ˆ yâ‚‚ â†’ (xâ‚ + yâ‚) â‰ˆ (xâ‚‚ + yâ‚‚)
    +-lunit : âˆ€ {x} â†’ (Îµ + x) â‰ˆ x
    +-assoc : âˆ€ {x y z} â†’ ((x + y) + z) â‰ˆ (x + (y + z))
    +-comm  : âˆ€ {x y} â†’ (x + y) â‰ˆ (y + x)

record _=[_]>_ {o e}{A B : Setoid o e}(X : CommutativeMonoid A)(f : A â‡’s B)(Y : CommutativeMonoid B) : Prop (o âŠ” e) where
  private
    module X = CommutativeMonoid X
    module Y = CommutativeMonoid Y
  open _â‡’s_ f
  open Setoid B
  field
    preserve-Îµ : func X.Îµ â‰ˆ Y.Îµ
    preserve-+ : âˆ€ {xâ‚ xâ‚‚} â†’ func (xâ‚ X.+ xâ‚‚) â‰ˆ (func xâ‚ Y.+ func xâ‚‚)
open _=[_]>_

module _ where

  open CommutativeMonoid

  ğŸ™cm : âˆ€ {o e} â†’ CommutativeMonoid (ğŸ™ {o} {e})
  ğŸ™cm .Îµ = lift tt
  ğŸ™cm ._+_ _ _ = lift tt
  ğŸ™cm .+-cong _ _ = tt
  ğŸ™cm .+-lunit = tt
  ğŸ™cm .+-assoc = tt
  ğŸ™cm .+-comm = tt

  _âŠ—_ : âˆ€ {o e}{A B : Setoid o e} â†’
        CommutativeMonoid A â†’
        CommutativeMonoid B â†’
        CommutativeMonoid (âŠ—-setoid A B)
  (X âŠ— Y) .Îµ = X .Îµ , Y .Îµ
  (X âŠ— Y) ._+_ (xâ‚ , yâ‚) (xâ‚‚ , yâ‚‚) = X ._+_ xâ‚ xâ‚‚ , Y ._+_ yâ‚ yâ‚‚
  (X âŠ— Y) .+-cong (xâ‚â‰ˆxâ‚‚ , yâ‚â‰ˆyâ‚‚) (x'â‚â‰ˆx'â‚‚ , y'â‚â‰ˆy'â‚‚) =
     X .+-cong xâ‚â‰ˆxâ‚‚ x'â‚â‰ˆx'â‚‚ , Y .+-cong yâ‚â‰ˆyâ‚‚ y'â‚â‰ˆy'â‚‚
  (X âŠ— Y) .+-lunit = X .+-lunit , Y .+-lunit
  (X âŠ— Y) .+-assoc = X .+-assoc , Y .+-assoc
  (X âŠ— Y) .+-comm = X .+-comm , Y .+-comm
